TimedKt.lean
@@ -19,4 +19,5 @@ import TimedKt.Kt
 import TimedKt.WriteOnce
 import TimedKt.InfoTransfer
 import TimedKt.BitCost
+import TimedKt.Triangle
 import TimedKt.Examples
